ArkLib/OracleReduction/Execution.lean
@@ -10,9 +10,9 @@ import ArkLib.Data.Fin.Basic
 
 open OracleComp OracleSpec SubSpec ProtocolSpec
 
-namespace loggingOracle
+universe u v
 
-universe u
+namespace loggingOracle
 
 variable {ι : Type u} {spec : OracleSpec ι} {α β : Type u}
 
@@ -32,6 +32,30 @@ theorem simulateQ_map_fst (oa : OracleComp spec α) :
 @[simp]
 theorem simulateQ_bind_fst (oa : OracleComp spec α) (f : α → OracleComp spec β) :
     (do let a ← (simulateQ loggingOracle oa).run; f a.1) = oa >>= f := by
+  induction oa using OracleComp.induction with
+  | pure a => simp
+  | query_bind i t oa ih => simp [simulateQ_bind, ih]
+  | failure => simp
+
+/-- We often have to specify `oa` and `f` for this to be applied -/
+theorem simulateQ_bind_fst_comp (oa : OracleComp spec α) (f : α → OracleComp spec β) :
+    (do let a ← (simulateQ loggingOracle oa).run; f a.1) = (do let a ← oa; f a) := by
+  induction oa using OracleComp.induction with
+  | pure a => simp
+  | query_bind i t oa ih => simp [simulateQ_bind, ih]
+  | failure => simp
+
+/-- Ideally, this theorem can also compare the logs of the two oracle computations.
+
+For this to work, we need an extra function mapping `superSpec.QueryLog` to `spec.QueryLog`.
+
+This function always exists if `superSpec` is `spec ++ₒ something`, and extensions thereof, but may
+not be guaranteed to exist in general, if we just have the current fields in the type class. -/
+@[simp]
+theorem simulateQ_run_liftComp_fst {ι' : Type u} {superSpec : OracleSpec ι'}
+    (oa : OracleComp spec α) [SubSpec spec superSpec] :
+      Prod.fst <$> (simulateQ loggingOracle oa).run.liftComp superSpec =
+        Prod.fst <$> (simulateQ loggingOracle (oa.liftComp superSpec)).run := by
   induction oa using OracleComp.induction with
   | pure a => simp
   | query_bind i t oa ih => simp [simulateQ_bind, ih]
@@ -61,7 +85,7 @@ def Prover.processRound (j : Fin n)
   match hDir : pSpec.getDir j with
   | .V_to_P => do
     let challenge ← pSpec.getChallenge ⟨j, hDir⟩
-    letI newState := prover.receiveChallenge ⟨j, hDir⟩ state challenge
+    letI newState := (← prover.receiveChallenge ⟨j, hDir⟩ state) challenge
     return ⟨transcript.concat challenge, newState⟩
   | .P_to_V => do
     let ⟨msg, newState⟩ ← prover.sendMessage ⟨j, hDir⟩ state
@@ -82,22 +106,20 @@ def Prover.runToRound (i : Fin (n + 1))
 
 /-- Run the prover in an interactive reduction up to round `i`, logging all the queries made by the
   prover. Returns the transcript up to that round, the prover's state after that round, and the log
-  of the prover's oracle queries.
+  of the prover's oracle queries. This basically just wraps `Prover.runToRound` with a logging
+  oracle.
 -/
 @[inline, specialize]
 def Prover.runWithLogToRound (i : Fin (n + 1))
     (stmt : StmtIn) (wit : WitIn) (prover : Prover oSpec StmtIn WitIn StmtOut WitOut pSpec) :
       OracleComp (oSpec ++ₒ [pSpec.Challenge]ₒ)
-        (pSpec.Transcript i × prover.PrvState i × QueryLog (oSpec ++ₒ [pSpec.Challenge]ₒ)) := do
-  let ⟨⟨transcript, state⟩, proveQueryLog⟩ ←
-    (simulateQ loggingOracle (prover.runToRound i stmt wit)).run
-  return ⟨transcript, state, proveQueryLog⟩
+        ((pSpec.Transcript i × prover.PrvState i) × QueryLog (oSpec ++ₒ [pSpec.Challenge]ₒ)) :=
+  (simulateQ loggingOracle (prover.runToRound i stmt wit)).run
 
 @[simp]
 lemma Prover.runWithLogToRound_discard_log_eq_runToRound (i : Fin (n + 1))
     (stmt : StmtIn) (wit : WitIn) (prover : Prover oSpec StmtIn WitIn StmtOut WitOut pSpec) :
-      (fun ⟨transcript, state, _⟩ => (transcript, state)) <$>
-        prover.runWithLogToRound i stmt wit = prover.runToRound i stmt wit := by
+      Prod.fst <$> prover.runWithLogToRound i stmt wit = prover.runToRound i stmt wit := by
   simp [runWithLogToRound, runToRound]
 
 /-- Run the prover in an interactive reduction. Returns the output statement and witness, and the
@@ -107,31 +129,30 @@ lemma Prover.runWithLogToRound_discard_log_eq_runToRound (i : Fin (n + 1))
 @[inline, specialize]
 def Prover.run (stmt : StmtIn) (wit : WitIn)
     (prover : Prover oSpec StmtIn WitIn StmtOut WitOut pSpec) :
-      OracleComp (oSpec ++ₒ [pSpec.Challenge]ₒ) ((StmtOut × WitOut) × FullTranscript pSpec) := do
+      OracleComp (oSpec ++ₒ [pSpec.Challenge]ₒ) (FullTranscript pSpec × StmtOut × WitOut) := do
   let ⟨transcript, state⟩ ← prover.runToRound (Fin.last n) stmt wit
-  return ⟨prover.output state, transcript⟩
+  return ⟨transcript, ← prover.output state⟩
 
 /-- Run the prover in an interactive reduction, logging all the queries made by the prover. Returns
-  the output statement and witness, the transcript, and the log of the prover's oracle queries.
+  the transcript, the output statement and witness, and the log of the prover's oracle queries.
+
+  Note: this is just a wrapper around `Prover.run` that logs the queries made by the prover.
 -/
-@[inline, specialize]
+@[inline, specialize, reducible]
 def Prover.runWithLog (stmt : StmtIn) (wit : WitIn)
     (prover : Prover oSpec StmtIn WitIn StmtOut WitOut pSpec) :
       OracleComp (oSpec ++ₒ [pSpec.Challenge]ₒ)
-        ((StmtOut × WitOut) × FullTranscript pSpec × QueryLog (oSpec ++ₒ [pSpec.Challenge]ₒ)) := do
-  let ⟨transcript, state, proveQueryLog⟩ ← prover.runWithLogToRound (Fin.last n) stmt wit
-  return ⟨prover.output state, transcript, proveQueryLog⟩
+        ((FullTranscript pSpec × StmtOut × WitOut) × QueryLog (oSpec ++ₒ [pSpec.Challenge]ₒ)) :=
+  (simulateQ loggingOracle (prover.run stmt wit)).run
 
 @[simp]
 lemma Prover.runWithLog_discard_log_eq_run (stmt : StmtIn) (wit : WitIn)
     (prover : Prover oSpec StmtIn WitIn StmtOut WitOut pSpec) :
-      (fun ⟨prvOutput, transcript, _⟩ => (prvOutput, transcript)) <$>
-        prover.runWithLog stmt wit = prover.run stmt wit := by
-  simp [run, runWithLog, ← runWithLogToRound_discard_log_eq_runToRound]
+      Prod.fst <$> prover.runWithLog stmt wit = prover.run stmt wit := by
+  simp [Prover.runWithLog]
 
 /-- Run the (non-oracle) verifier in an interactive reduction. It takes in the input statement and
-  the transcript, and return the output statement along with the log of oracle queries made by the
-  veirifer.
+  the transcript, and return the output statement.
 -/
 @[inline, specialize, reducible]
 def Verifier.run (stmt : StmtIn) (transcript : FullTranscript pSpec)
@@ -164,8 +185,8 @@ theorem OracleVerifier.run_eq_run_verifier [Oₘ : ∀ i, OracleInterface (pSpec
   rfl
 
 /-- An execution of an interactive reduction on a given initial statement and witness. Consists of
-  first running the prover, and then the verifier. Returns the output statement and witness, and the
-  full transcript.
+  first running the prover, and then the verifier. Returns the full transcript, the output statement
+  and witness from the prover, and the output statement from the verifier.
 
   See `Reduction.runWithLog` for a version that additionally returns the logs of the prover's and
   the verifier's oracle queries.
@@ -174,39 +195,59 @@ theorem OracleVerifier.run_eq_run_verifier [Oₘ : ∀ i, OracleInterface (pSpec
 def Reduction.run (stmt : StmtIn) (wit : WitIn)
     (reduction : Reduction oSpec StmtIn WitIn StmtOut WitOut pSpec) :
       OracleComp (oSpec ++ₒ [pSpec.Challenge]ₒ)
-        ((StmtOut × WitOut) × StmtOut × FullTranscript pSpec) := do
+        ((FullTranscript pSpec × StmtOut × WitOut) × StmtOut) := do
   -- `ctxOut` contains both the output statement and witness after running the prover
-  let ⟨ctxOut, transcript⟩ ← reduction.prover.run stmt wit
-  let stmtOut ← liftM (reduction.verifier.run stmt transcript)
-  return (ctxOut, stmtOut, transcript)
+  let proverResult ← reduction.prover.run stmt wit
+  let stmtOut ← liftM (reduction.verifier.run stmt proverResult.1)
+  return ⟨proverResult, stmtOut⟩
 
 /-- An execution of an interactive reduction on a given initial statement and witness. Consists of
-  first running the prover, and then the verifier. Returns the output statement and witness, the
-  full transcript, and the logs of the prover's and the verifier's oracle queries.
+  first running the prover, and then the verifier. Returns the full transcript, the output statement
+  and witness from the prover, and the output statement from the verifier, along with the logs of
+  the prover's and the verifier's oracle queries.
 -/
 @[inline, specialize]
 def Reduction.runWithLog (stmt : StmtIn) (wit : WitIn)
     (reduction : Reduction oSpec StmtIn WitIn StmtOut WitOut pSpec) :
       OracleComp (oSpec ++ₒ [pSpec.Challenge]ₒ)
-        ((StmtOut × WitOut) × StmtOut × FullTranscript pSpec ×
+        (((FullTranscript pSpec × StmtOut × WitOut) × StmtOut) ×
           QueryLog (oSpec ++ₒ [pSpec.Challenge]ₒ) × QueryLog oSpec) := do
   -- `ctxOut` contains both the output statement and witness after running the prover
-  let ⟨ctxOut, transcript, proveQueryLog⟩ ← reduction.prover.runWithLog stmt wit
+  let ⟨proverResult, proveQueryLog⟩ ← reduction.prover.runWithLog stmt wit
   let ⟨stmtOut, verifyQueryLog⟩ ←
-    liftM (simulateQ loggingOracle (reduction.verifier.run stmt transcript)).run
-  return (ctxOut, stmtOut, transcript, proveQueryLog, verifyQueryLog)
+    liftM (simulateQ loggingOracle (reduction.verifier.run stmt proverResult.1)).run
+  return ⟨⟨proverResult, stmtOut⟩, proveQueryLog, verifyQueryLog⟩
+
+/-- TODO: figure out a better name for this -/
+private lemma Monad.map_of_prod_fst_eq_prod_fst {m : Type u → Type v} [Monad m] [LawfulMonad m]
+    {α β γ : Type u} (ma : m (α × β)) (c : γ) :
+    (fun a => (c, a.1)) <$> ma = Prod.mk c <$> Prod.fst <$> ma := by
+  simp only [Functor.map_map]
 
 /-- Logging the queries made by both parties do not change the output of the reduction -/
 @[simp]
 theorem Reduction.runWithLog_discard_logs_eq_run
     {stmt : StmtIn} {wit : WitIn}
     {reduction : Reduction oSpec StmtIn WitIn StmtOut WitOut pSpec} :
-      (fun ⟨prvOutput, witOut, transcript, _, _⟩ => (prvOutput, witOut, transcript)) <$>
+      Prod.fst <$>
         reduction.runWithLog stmt wit = reduction.run stmt wit := by
-  simp [run, runWithLog, Verifier.run, ← Prover.runWithLog_discard_log_eq_run]
-  congr
-  simp_rw [map_eq_pure_bind]
-  sorry
+  simp [runWithLog, run, Prover.runWithLog]
+  set proverRun := Prover.run stmt wit reduction.prover
+  calc
+  _ = (do
+    let a ← (simulateQ loggingOracle proverRun).run
+    (fun aFst : (pSpec.FullTranscript × StmtOut × WitOut) => (fun b => (aFst, Prod.fst b)) <$>
+        (simulateQ loggingOracle (Verifier.run stmt aFst.1 reduction.verifier)).run.liftComp
+          (oSpec ++ₒ [pSpec.Challenge]ₒ)) a.1) := rfl
+  _ = _ := by
+    rw [loggingOracle.simulateQ_bind_fst_comp proverRun
+      (fun a => (fun b => (a, Prod.fst b)) <$>
+        (simulateQ loggingOracle (Verifier.run stmt a.1 reduction.verifier)).run.liftComp
+          (oSpec ++ₒ [pSpec.Challenge]ₒ))]
+    congr
+    ext proverResult
+    rw [← Functor.map_map]
+    simp
 
 /-- Run an interactive oracle reduction. Returns the full transcript, the output statement and
   witness, the log of all prover's oracle queries, and the log of all verifier's oracle queries to
@@ -217,11 +258,11 @@ def OracleReduction.run [∀ i, OracleInterface (pSpec.Message i)]
     (stmt : StmtIn) (oStmt : ∀ i, OStmtIn i) (wit : WitIn)
     (reduction : OracleReduction oSpec StmtIn OStmtIn WitIn StmtOut OStmtOut WitOut pSpec) :
       OracleComp (oSpec ++ₒ [pSpec.Challenge]ₒ)
-        (((StmtOut × ∀ i, OStmtOut i) × WitOut) × (StmtOut × ∀ i, OStmtOut i)
-          × FullTranscript pSpec) := do
-  let ⟨ctxOut, transcript⟩ ← reduction.prover.run ⟨stmt, oStmt⟩ wit
-  let stmtOut ← liftM (reduction.verifier.run stmt oStmt transcript)
-  return (ctxOut, stmtOut, transcript)
+        ((FullTranscript pSpec × (StmtOut × ∀ i, OStmtOut i) × WitOut) ×
+          (StmtOut × ∀ i, OStmtOut i)) := do
+  let proverResult ← reduction.prover.run ⟨stmt, oStmt⟩ wit
+  let stmtOut ← liftM (reduction.verifier.run stmt oStmt proverResult.1)
+  return ⟨proverResult, stmtOut⟩
 
 /-- Run an interactive oracle reduction. Returns the full transcript, the output statement and
   witness, the log of all prover's oracle queries, and the log of all verifier's oracle queries to
@@ -232,13 +273,14 @@ def OracleReduction.runWithLog [∀ i, OracleInterface (pSpec.Message i)]
     (stmt : StmtIn) (oStmt : ∀ i, OStmtIn i) (wit : WitIn)
     (reduction : OracleReduction oSpec StmtIn OStmtIn WitIn StmtOut OStmtOut WitOut pSpec) :
       OracleComp (oSpec ++ₒ [pSpec.Challenge]ₒ)
-        (((StmtOut × ∀ i, OStmtOut i) × WitOut) × (StmtOut × ∀ i, OStmtOut i)
-          × FullTranscript pSpec × QueryLog (oSpec ++ₒ [pSpec.Challenge]ₒ) × QueryLog oSpec) := do
-  let ⟨⟨ctxOut, transcript⟩, proveQueryLog⟩ ←
+        ((FullTranscript pSpec × (StmtOut × ∀ i, OStmtOut i) × WitOut) ×
+          (StmtOut × ∀ i, OStmtOut i) ×
+            QueryLog (oSpec ++ₒ [pSpec.Challenge]ₒ) × QueryLog oSpec) := do
+  let ⟨proverResult, proveQueryLog⟩ ←
     (simulateQ loggingOracle (reduction.prover.run ⟨stmt, oStmt⟩ wit)).run
   let ⟨stmtOut, verifyQueryLog⟩ ←
-    liftM (simulateQ loggingOracle (reduction.verifier.run stmt oStmt transcript)).run
-  return (ctxOut, stmtOut, transcript, proveQueryLog, verifyQueryLog)
+    liftM (simulateQ loggingOracle (reduction.verifier.run stmt oStmt proverResult.1)).run
+  return ⟨proverResult, stmtOut, proveQueryLog, verifyQueryLog⟩
 
 /-- Running an oracle reduction is equal to running its non-oracle counterpart -/
 @[simp]
@@ -283,7 +325,7 @@ section Trivial
 @[simp]
 theorem Reduction.id_run (stmt : StmtIn) (wit : WitIn) :
     (Reduction.id : Reduction oSpec StmtIn WitIn _ _ _).run stmt wit =
-      pure ⟨⟨stmt, wit⟩, stmt, default⟩ := by
+      pure ⟨⟨default, stmt, wit⟩, stmt⟩ := by
   simp [Reduction.run, Reduction.id, Prover.run, Verifier.run, Prover.id, Verifier.id]
 
 /-- Running the identity or trivial reduction, with logging of queries to the shared oracle,
@@ -291,8 +333,8 @@ theorem Reduction.id_run (stmt : StmtIn) (wit : WitIn) :
 @[simp]
 theorem Reduction.id_runWithLog (stmt : StmtIn) (wit : WitIn) :
     (Reduction.id : Reduction oSpec StmtIn WitIn _ _ _).runWithLog stmt wit =
-      pure ⟨⟨stmt, wit⟩, stmt, default, [], []⟩ := by
-  simp [Reduction.runWithLog, Reduction.id, Prover.runWithLog, Prover.runWithLogToRound,
+      pure ⟨⟨⟨default, stmt, wit⟩, stmt⟩, [], []⟩ := by
+  simp [Reduction.runWithLog, Reduction.id, Prover.runWithLog, Prover.run,
     Verifier.run, Prover.id, Verifier.id]
 
 /-- Running the identity or trivial oracle reduction results in the same input statement, oracle
@@ -300,7 +342,7 @@ theorem Reduction.id_runWithLog (stmt : StmtIn) (wit : WitIn) :
 @[simp]
 theorem OracleReduction.id_run (stmt : StmtIn) (oStmt : ∀ i, OStmtIn i) (wit : WitIn) :
     (OracleReduction.id : OracleReduction oSpec StmtIn OStmtIn WitIn _ _ _ _).run stmt oStmt wit =
-      pure ⟨⟨⟨stmt, oStmt⟩, wit⟩, ⟨stmt, oStmt⟩, default⟩ := by
+      pure ⟨⟨default, ⟨stmt, oStmt⟩, wit⟩, ⟨stmt, oStmt⟩⟩ := by
   simp [OracleReduction.run, OracleVerifier.run,
     Prover.run, OracleReduction.id, OracleProver.id, OracleVerifier.id, Prover.id]
 
@@ -309,7 +351,7 @@ theorem OracleReduction.id_run (stmt : StmtIn) (oStmt : ∀ i, OStmtIn i) (wit :
 @[simp]
 theorem OracleReduction.id_runWithLog (stmt : StmtIn) (oStmt : ∀ i, OStmtIn i) (wit : WitIn) :
     (OracleReduction.id : OracleReduction oSpec StmtIn OStmtIn WitIn _ _ _ _).runWithLog
-      stmt oStmt wit = pure ⟨⟨⟨stmt, oStmt⟩, wit⟩, ⟨stmt, oStmt⟩, default, [], []⟩ := by
+      stmt oStmt wit = pure ⟨⟨default, ⟨stmt, oStmt⟩, wit⟩, ⟨stmt, oStmt⟩, [], []⟩ := by
   simp [OracleReduction.runWithLog, OracleVerifier.run,
     Prover.run, OracleReduction.id, OracleProver.id, OracleVerifier.id, Prover.id]
 
@@ -343,25 +385,21 @@ theorem Prover.run_of_prover_first [ProverOnly pSpec] (stmt : StmtIn) (wit : Wit
       prover.run stmt wit = (do
         let state := prover.input (stmt, wit)
         let ⟨msg, state⟩ ← liftComp (prover.sendMessage ⟨0, by simp⟩ state) _
-        let ctxOut := prover.output state
-        return (ctxOut, fun i => match i with | ⟨0, _⟩ => msg)) := by
+        let ctxOut ← prover.output state
+        return ((fun i => match i with | ⟨0, _⟩ => msg), ctxOut)) := by
   simp [Prover.run]; rfl
 
-@[simp]
+-- @[simp]
 theorem Reduction.run_of_prover_first [ProverOnly pSpec] (stmt : StmtIn) (wit : WitIn)
     (reduction : Reduction oSpec StmtIn WitIn StmtOut WitOut pSpec) :
       reduction.run stmt wit = (do
         let state := reduction.prover.input (stmt, wit)
         let ⟨msg, state⟩ ← liftComp (reduction.prover.sendMessage ⟨0, by simp⟩ state) _
-        let (prvStmtOut, witOut) := reduction.prover.output state
+        let ctxOut ← reduction.prover.output state
         let transcript : pSpec.FullTranscript := fun i => match i with | ⟨0, _⟩ => msg
         let stmtOut ← reduction.verifier.verify stmt transcript
-        return ((prvStmtOut, witOut), stmtOut, transcript)) := by
+        return (⟨transcript, ctxOut⟩, stmtOut)) := by
   simp [Reduction.run, Verifier.run, ← liftComp_map]
-  conv =>
-    enter [1, 1]
-    rw [map_eq_pure_bind]
-    simp
   -- conv =>
   --   enter [1, 2, a, 1]
   --   rw [map_eq_pure_bind]
